Submission 1

HW 7/LoVe02_ProgramsAndTheorems_ExerciseSheet.lean
@@ -23,7 +23,8 @@ its argument, or 0 if the argument is 0. For example:
     `pred 0 = 0` -/
 
 def pred : ℕ → ℕ :=
-  sorry
+  | 0       => 0
+  | n + 1   => n
 
 /- 1.2. Check that your function works as expected. -/
 
@@ -62,6 +63,15 @@ def someEnv : String → ℤ
 
 #eval eval someEnv (AExp.var "x")   -- expected: 3
 -- invoke `#eval` here
+#eval eval someEnv (AExp.add 2 3)
+#eval eval someEnv (AExp.sub 7 4)
+#eval eval someEnv (AExp.mul 5 3)
+#eval eval someEnv (AExp.div 12 4)
+#eval eval someEnv (AExp.div 6 0)
+#eval eval someEnv (AExp.num 9)
+
+
+
 
 /- 2.2. The following function simplifies arithmetic expressions involving
 addition. It simplifies `0 + e` and `e + 0` to `e`. Complete the definition so
@@ -72,6 +82,12 @@ def simplify : AExp → AExp
   | AExp.add (AExp.num 0) e₂ => simplify e₂
   | AExp.add e₁ (AExp.num 0) => simplify e₁
   -- insert the missing cases here
+  | AExp.sub e₁ (AExp.num 0) => simplify e₁
+  | AExp.mul (AExp.num 1) e₂ => simplify e₂
+  | AExp.mul e₁ (AExp.num 1) => simplify e₁
+  | AExp.mul (AExp.num 0) e₂ => simplify 0
+  | AExp.mul e₁ (AExp.num 0) => simplify 0
+  | AExp.div e₁ (AExp.num 1) => simplify e₁
   -- catch-all cases below
   | AExp.num i               => AExp.num i
   | AExp.var x               => AExp.var x
@@ -90,7 +106,7 @@ the property that the value of `e` after simplification is the same as the
 value of `e` before. -/
 
 theorem simplify_correct (env : String → ℤ) (e : AExp) :
-  True :=   -- replace `True` by your theorem statement
+  eval env (simplify e) = eval e :=   -- replace `True` by your theorem statement
   sorry   -- leave `sorry` alone
 
 
@@ -100,7 +116,8 @@ theorem simplify_correct (env : String → ℤ) (e : AExp) :
 every element in a list. -/
 
 def map {α : Type} {β : Type} (f : α → β) : List α → List β :=
-  sorry
+  | []        => []
+  | x :: xs   => f x :: map f xs
 
 #eval map (fun n ↦ n + 10) [1, 2, 3]   -- expected: [11, 12, 13]
 
@@ -114,5 +131,12 @@ Try to give meaningful names to your theorems. Also, make sure to state the
 second property as generally as possible, for arbitrary types. -/
 
 -- enter your theorem statements here
+theorem MapIdentityFunction (xs : List α) :
+  map (fun x ↦ x) xs = xs :=
+  sorry
+
+theorem Composition (xs : List α) (f : α → β) (g : β → γ):
+  map (fun x ↦ g (f x)) xs = map g (map f xs) :=
+  sorry
 
 end LoVe
