HW 7/Exercises/Exercises.lean
@@ -1,1 +1,0 @@
-import Exercises.Basic
