HW 7/LoVe01_TypesAndTerms_ExerciseSheet.lean
@@ -32,18 +32,18 @@ def K : α → β → α :=
   fun a b ↦ a
 
 def C : (α → β → γ) → β → α → γ :=
-  sorry
+  fun f a b ↦ f b a
 
 def projFst : α → α → α :=
-  sorry
+  fun a1 a2 ↦ a1
 
 /- Give a different answer than for `projFst`. -/
 
 def projSnd : α → α → α :=
-  sorry
+  fun a1 a2 ↦ a2
 
 def someNonsense : (α → β → γ) → α → (α → γ) → β → γ :=
-  sorry
+  fun f1 a f2 b ↦ f a b
 
 
 /- ## Question 2: Typing Derivation
